formic_site_duct/formic.apis.duct.dfy
@@ -5,16 +5,22 @@ module DuctApis {
 
     class Views {
         static method Endpoints() returns (all: AllApiEndpoints)
-            ensures |all.endpoints| == 1
         {
             var catalog := new AllApiEndpoints();
 
             var formic_landing := new FormicLandingPage();
-            var ep := new ApiEndpoint("/", ReturnType.Content, formic_landing);
-            catalog.Add(ep);
+            var home := new ApiEndpoint("/", ReturnType.Content(""), formic_landing);
+            catalog.Add(home);
 
+            var login_page := new LoginChallengePage();
+            var login := new ApiEndpoint("/login", ReturnType.ChallengeGoogle("/"), login_page);
+            catalog.Add(login);
+
+            var secure_page := new SecurePage();
+            var secure := new ApiEndpoint("/secure", ReturnType.Content(""), secure_page);
+            catalog.Add(secure);
+            
             all := catalog;
         }
     }
-
 }
